minuska/theories/default_everything.v
@@ -34,26 +34,30 @@ Proof.
 Defined.
 
 #[export]
-Instance DSM {β : Builtin MyUnit} : StaticModel :=
-    default_model β
+Instance DSM
+    {β : Builtin MyUnit}
+    (program_info : ProgramInfo)
+    : StaticModel :=
+    default_model β program_info
 .
 
 Definition GT {β : Builtin MyUnit} := @TermOver' string (builtin_value).
 
-Definition StepT {β : Builtin MyUnit} := NondetValue -> GT -> option GT.
-Definition StepT_ext {β : Builtin MyUnit} := NondetValue -> GT -> option (GT*nat).
+Definition StepT {β : Builtin MyUnit} (program_info : ProgramInfo) := NondetValue -> GT -> option GT.
+Definition StepT_ext {β : Builtin MyUnit} (program_info : ProgramInfo) := NondetValue -> GT -> option (GT*nat).
 
 Definition gt_over {β : Builtin MyUnit} (b : builtin_value) : GT := @t_over string builtin_value b.
 Definition gt_term {β : Builtin MyUnit} (s : string) (l : list GT) : GT := @t_term string builtin_value s l.
 
 Definition basic_rule
     {β : Builtin MyUnit}
+    (program_info : ProgramInfo)
     (name : string)
     (l : TermOver BuiltinOrVar)
     (r : TermOver Expression2)
     (conds : list SideCondition2) : Declaration
 :=
-    (decl_rule (@mkRuleDeclaration DSM Act name (@mkRewritingRule2 DSM Act l r conds default_act)))
+    (decl_rule (@mkRuleDeclaration (DSM program_info) Act name (@mkRewritingRule2 (DSM program_info) Act l r conds default_act)))
 .
 
 
@@ -70,19 +74,36 @@ Definition BoV_to_Expr2
 
 Definition framed_rule
     {β : Builtin MyUnit}
+    (program_info : ProgramInfo)
     (frame : (variable*(TermOver BuiltinOrVar)))
     (name : string)
     (l : TermOver BuiltinOrVar)
     (r : TermOver Expression2)
     (conds : list SideCondition2) : Declaration
 :=
-    (decl_rule (@mkRuleDeclaration DSM Act name (@mkRewritingRule2 DSM Act
+    (decl_rule (@mkRuleDeclaration (DSM program_info) Act name (@mkRewritingRule2 (DSM program_info) Act
         (TermOverBoV_subst frame.2 frame.1 l)
         (TermOverBoV_subst_expr2 frame.2 frame.1 r)
         conds default_act)))
 .
 
-Definition global_naive_interpreter {β : Builtin MyUnit} := @naive_interpreter DSM Act.
-Definition global_naive_interpreter_ext {β : Builtin MyUnit} := @naive_interpreter_ext DSM Act.
-Definition global_naive_interpreter_sound {β : Builtin MyUnit} := @naive_interpreter_sound DSM Act.
-(* Definition builtins_binding {β : Builtin MyUnit} := Minuska.builtins.builtins_binding. *)
+Definition global_naive_interpreter
+    {β : Builtin MyUnit}
+    (program_info : ProgramInfo)
+    :=
+    @naive_interpreter (DSM program_info) Act
+.
+
+Definition global_naive_interpreter_ext
+    {β : Builtin MyUnit}
+    (program_info : ProgramInfo)
+    :=
+    @naive_interpreter_ext (DSM program_info) Act
+.
+
+Definition global_naive_interpreter_sound
+    {β : Builtin MyUnit}
+    (program_info : ProgramInfo)
+    :=
+    @naive_interpreter_sound (DSM program_info) Act
+.
