minuska/theories/minusl_semantics.v
@@ -15,6 +15,7 @@ Section MinusL_sem.
 
     Inductive MinusL_rewrites
         (D : MinusL_LangDef Act)
+        (program : ProgramT)
         :
         (TermOver builtin_value) ->
         (TermOver builtin_value) ->
@@ -25,7 +26,7 @@ Section MinusL_sem.
 
     | mlr_refl :
         forall ctrl state,
-            MinusL_rewrites D ctrl state [] ctrl state
+            MinusL_rewrites D program ctrl state [] ctrl state
 
     | mlr_rule : 
         forall
@@ -38,18 +39,18 @@ Section MinusL_sem.
             (ρ : Valuation2),
             satisfies ρ ctrl1 lc ->
             satisfies ρ state1 ld ->
-            satisfies ρ (nv,ctrl2) rc ->
-            satisfies ρ (nv,state2) rd ->
-            satisfies ρ nv scs ->
-        MinusL_rewrites D ctrl1 state1 [a] ctrl2 state2
+            satisfies ρ (program, (nv,ctrl2)) rc ->
+            satisfies ρ (program, (nv,state2)) rd ->
+            satisfies ρ (program, nv) scs ->
+        MinusL_rewrites D program ctrl1 state1 [a] ctrl2 state2
 
     | mlr_trans :
         forall
             (ctrl1 state1 ctrl2 state2 ctrl3 state3 : TermOver builtin_value)
             (w1 w2 : list Act),
-        MinusL_rewrites D ctrl1 state1 w1 ctrl2 state2 ->
-        MinusL_rewrites D ctrl2 state2 w2 ctrl3 state3 ->
-        MinusL_rewrites D ctrl1 state1 (w1 ++ w2) ctrl3 state3
+        MinusL_rewrites D program ctrl1 state1 w1 ctrl2 state2 ->
+        MinusL_rewrites D program ctrl2 state2 w2 ctrl3 state3 ->
+        MinusL_rewrites D program ctrl1 state1 (w1 ++ w2) ctrl3 state3
 
     | mlr_context :
         forall
@@ -64,11 +65,11 @@ Section MinusL_sem.
             (nv : NondetValue),
             (∀ x, x ∈ vars_of_to_l2r c -> x <> h -> ρ1 !! x = ρ2 !! x) ->
             satisfies (<[h := r]>ρ1) ctrl1 c ->
-            satisfies ρ1 nv scs ->
+            satisfies ρ1 (program, nv) scs ->
             satisfies (<[h := v]>ρ2) ctrl2 c ->
-            satisfies ρ2 nv (MinusL_isValue Act D (e_ground v)) ->
-            MinusL_rewrites D r state1 w v state2 ->
-            MinusL_rewrites D ctrl1 state1 w ctrl2 state2
+            satisfies ρ2 (program, nv) (MinusL_isValue Act D (e_ground v)) ->
+            MinusL_rewrites D program r state1 w v state2 ->
+            MinusL_rewrites D program ctrl1 state1 w ctrl2 state2
     .
 
 End MinusL_sem.
